Jon defers a conflict

concurrency/node-replication/rwlock/Impl.i.dfy
@@ -1,5 +1,23 @@
+include "../../framework/Atomic.s.dfy"
+include "../../framework/Cells.s.dfy"
+include "../../../lib/Lang/LinearSequence.i.dfy"
+include "RwLock.i.dfy"
+
 module RwLockImpl {
-  // TODO implement this
+  import opened RwLockToken
+  import opened Atomics
+  import opened LinearSequence_s
+  import opened LinearSequence_i
+  import opened Cells
+  import opened GhostLoc
+  import opened GlinearOption
+
+  import RwLockMod = RwLock
+  import Handle
+
+  // We wish that V were a type parameter, but we don't actually have
+  // type parameters.
+  type V = Handle.Handle
 
   /*
    * Constructor for a new mutex.
@@ -11,8 +29,8 @@ module RwLockImpl {
    *     behind this mutex.
    */
 
-  method {:extern} new_mutex<V>(glinear v: V, ghost inv: (V) -> bool)
-  returns (m: RwLock<V>)
+  method new_mutex(glinear v: V, ghost inv: (V) -> bool)
+  returns (m: RwLock)
   requires inv(v)
   ensures m.inv == inv
 
@@ -24,7 +42,7 @@ module RwLockImpl {
    * calls a `release` without previously calling `acquire`.
    */
 
-  datatype ExclusiveGuard<V> = ExclusiveGuard(ghost m: RwLock<V>)
+  datatype ExclusiveGuard = ExclusiveGuard(ghost m: RwLock)
 
   /*
    * A SharedGuard is for shared access.
@@ -32,15 +50,40 @@ module RwLockImpl {
    * to the data structure stored in the mutex.
    */
 
-  datatype SharedGuard<V> = SharedGuard(ghost m: RwLock<V>, ghost v: V)
+  datatype SharedGuard = SharedGuard(ghost m: RwLock, ghost v: V)
 
   /*
    * RwLock that protects a piece of data with some invariant.
    */
 
-  type {:extern} RwLock(==)<!V>
+  linear datatype RwLock = RwLock(
+    linear exclusiveFlag: Atomic<bool, Token>,  // implements ExclusiveState.exc
+    linear refCounts: lseq<Atomic<nat, Token>>,  // implements map<ThreadId, nat>
+    linear cell: Cell<Handle.ContentsType>,      // implements the actual value that ExclusiveState.shared_value represents
+    ghost loc: Loc                              // which instance of this lock we're talking about
+  )
   {
-    predicate {:extern} inv(v: V)
+    predicate inv(v: V)  // client's invariant
+
+    predicate InternalInv()
+    {
+      && (forall v, token :: atomic_inv(exclusiveFlag, v, token)
+            <==> (
+              && token.val.exclusive.ExclusiveState?          // Token has an ExclusiveState in it
+              && token.val == RwLockMod.CentralHandle(token.val.exclusive)  // Token doesn't have anything else in it
+              && v == token.val.exclusive.exc                 // Token lock state matches protected bool
+              && cell == token.val.exclusive.stored_value.cell  // Token stored value reflects what's in the cell
+              && token.loc == loc
+            )
+          )
+      && (forall t, count, token :: atomic_inv(refCounts[t], count, token)
+            <==> (
+              // Token is a single refcount that matches the protected count
+              && token.val == RwLockMod.RefCount(t, count)
+              && token.loc == loc
+              )
+          )
+    }
 
     /*
      * `acquire`
@@ -48,17 +91,73 @@ module RwLockImpl {
      * inside meets the invariant.
      */
 
-    method {:extern} acquire()
-    returns (glinear v: V, glinear handle: ExclusiveGuard<V>)
+    predicate IsPendingHandle(token: RwLockToken.Token, visited: int)
+    {
+      && token.val == RwLockMod.ExcHandle(token.val.exc)  // it's an ExcState
+      && token.val.exc.visited == visited
+      && token.val.exc.b.cell == this.cell
+      && token.loc == this.loc
+    }
+
+    shared method acquire()
+    returns (glinear v: V, glinear handle: ExclusiveGuard)
     ensures this.inv(v)
     ensures handle.m == this
+    decreases *
+    {
+      var got_exc := false;
+      glinear var pending_handle := RwLockToken.T.get_unit(this.loc);
+
+      while !got_exc
+      invariant got_exc ==> IsPendingHandle(pending_handle, 0)
+      decreases *
+      {
+        atomic_block got_exc := execute_atomic_compare_and_set_strong(this.exclusiveFlag, false, true) {
+          ghost_acquire g;
+          if got_exc {
+            RwLockToken.T.dispose(pending_handle);
+            g, pending_handle := RwLockToken.perform_ExcBegin(g);
+          }
+          ghost_release g;
+        }
+      }
+
+      var visited := 0;
+
+      while visited < RwLockMod.RC_WIDTH
+        invariant 0 <= visited < RwLockMod.RC_WIDTH
+        // if we find a nonzero refcount, we'll just keep waiting.
+        // (Deadlock breaking is the shared-acquirer's problem.)
+        invariant this.InternalInv()
+        invariant if visited==RwLockMod.RC_WIDTH
+          then pending_handle.val == RwLockMod.ExcHandle(RwLockMod.ExcObtained)
+          else IsPendingHandle(pending_handle, visited)
+        invariant pending_handle.loc == this.loc
+        decreases *
+      {
+        atomic_block var ret_value := execute_atomic_load(this.refCounts[visited]) {
+          ghost_acquire token_g; // the token in refCounts[visited]
+
+          if ret_value == 0 {
+            // If we find a zero, we advance visited
+            pending_handle, token_g := RwLockToken.perform_TakeExcLockCheckRefCount(pending_handle, token_g);
+            visited := visited + 1;
+          }
+          // else try checking this slot again; maybe a reader left. visited stays where it is.
+
+          ghost_release token_g;
+        }
+      }
+
+      handle := pending_handle;
+    }
 
     /*
      * `release`
      * The client must ensure that the data meets the invariant.
      */
 
-    method {:extern} release(glinear v: V, glinear handle: ExclusiveGuard<V>)
+    method release(glinear v: V, glinear handle: ExclusiveGuard)
     requires this.inv(v)
     requires handle.m == this
 
@@ -68,8 +167,13 @@ module RwLockImpl {
      * Returns a handle that can be borrowed from
      */
 
+<<<<<<< HEAD
     shared method acquire_shared()
     returns (linear handle: SharedGuard<V>)
+=======
+    method acquire_shared()
+    returns (linear handle: SharedGuard)
+>>>>>>> 58375053 (progress on rwlock/Impl)
     ensures this.inv(handle.v)
     ensures handle.m == this
 
@@ -77,11 +181,15 @@ module RwLockImpl {
      * `acquire_release`
      */
 
+<<<<<<< HEAD
     shared method release_shared(linear handle: SharedGuard<V>)
+=======
+    method release_shared(linear handle: SharedGuard)
+>>>>>>> 58375053 (progress on rwlock/Impl)
     requires handle.m == this
   }
 
-  function method {:extern} borrow_shared<V>(shared handle: SharedGuard<V>)
+  function method borrow_shared(shared handle: SharedGuard)
       : (shared v: V)
   ensures v == handle.v
 }
